checkpoint before switching styles

src/lib/kuiper/Kuiper.Array.Core.fst
@@ -42,13 +42,13 @@ returns x:a
 ensures post x
 { admit() }
 
-let gpu_array (a : Type u#0) (sz : nat) : Type u#0 = A.larray a sz
+let gpu_array_core (a : Type u#0) (sz : nat) : Type u#0 = A.larray a sz
 let loc_id_of_array #a #sz x = loc_id_of_array x
 let visibility_of #a #sz x = visibility_of_array x
 
 (* Base address of the GPU array, used to model alignment. This number
 is in units of *bytes*, not array elements. *)
-let base_address (#a : Type u#0) (#sz : nat) (x : gpu_array a sz)
+let base_address (#a : Type u#0) (#sz : nat) (x : gpu_array_core a sz)
 : GTot nat
 = core_base_address x
 
@@ -58,7 +58,7 @@ let mask_of (i j:nat) (n:nat) : prop = i <= n /\ n < j
 let gpu_pts_to_slice_core 
   (#a:Type u#0)
   (#sz:nat)
-  ([@@@mkey] x:gpu_array a sz)
+  ([@@@mkey] x:gpu_array_core a sz)
   (#[exact (`1.0R)] f : perm)
   ([@@@mkey] i : nat)
   (j : nat)
@@ -75,7 +75,7 @@ let gpu_pts_to_slice_core
 instance is_send_gpu_pts_to_slice_core 
   (#a:Type u#0)
   (#sz:nat)
-  ([@@@mkey] x:gpu_array a sz)
+  ([@@@mkey] x:gpu_array_core a sz)
   (#[exact (`1.0R)] f : perm)
   ([@@@mkey] i : nat)
   (j : nat)
@@ -88,7 +88,7 @@ instance is_send_gpu_pts_to_slice_core
 let gpu_pts_to_slice
   (#a:Type u#0)
   (#sz:nat)
-  ([@@@mkey] x:gpu_array a sz)
+  ([@@@mkey] x:gpu_array_core a sz)
   (#[exact (`1.0R)] f : perm)
   ([@@@mkey] i : nat)
   (j : nat)
@@ -99,7 +99,7 @@ let gpu_pts_to_slice
 let placeless_gpu_pts_to_slice
   (#a:Type u#0)
   (#sz:nat)
-  (x:gpu_array a sz)
+  (x:gpu_array_core a sz)
   (#[exact (`1.0R)] f : perm)
   (i : nat)
   (j : nat)
@@ -112,7 +112,7 @@ fn gpu_pts_to_slice_ref
   (#a:Type u#0)
   (#sz:nat)
   (#f : perm)
-  (x:gpu_array a sz)
+  (x:gpu_array_core a sz)
   (i:nat) (j:nat)
   (#v : seq a)
   preserves gpu_pts_to_slice x #f i j v
@@ -147,7 +147,7 @@ fn gpu_array_alloc_vis
   (l:loc_id)
   (vis:visibility)
   preserves cpu
-  returns   x : gpu_array a (SZ.v sz)
+  returns   x : gpu_array_core a (SZ.v sz)
   ensures
     exists* (s:seq a). x |-> s ** pure (Seq.length s == sz)
   ensures
@@ -159,7 +159,7 @@ fn gpu_array_alloc_vis
 {
   fn aux ()
   requires loc l ** dummy
-  returns  x : gpu_array a (SZ.v sz)
+  returns  x : gpu_array_core a (SZ.v sz)
   ensures loc l
   ensures exists* (s:seq a). 
     gpu_pts_to_array x s **
@@ -188,7 +188,7 @@ fn gpu_array_alloc
   {| d: sized a |}
   (sz : SZ.t)
   preserves cpu
-  returns   x : gpu_global_array a (SZ.v sz)
+  returns   x : gpu_array a (SZ.v sz)
   ensures
     exists* (s:seq a). x |-> s ** pure (Seq.length s == sz)
   ensures
@@ -202,7 +202,7 @@ fn gpu_array_alloc
 fn gpu_array_free
   (#a:Type u#0)
   (#sz:erased nat)
-  (r : gpu_array a sz)
+  (r : gpu_array_core a sz)
   (#v : erased (seq a))
   preserves cpu
   requires r |-> v
@@ -232,7 +232,7 @@ fn gpu_array_read_local
   (#sz : erased nat)
   (#i  : erased nat)
   (#j  : erased nat)
-  (r : gpu_array a sz)
+  (r : gpu_array_core a sz)
   (#f : perm)
   (idx : SZ.t)
   (#s : erased (seq a))
@@ -255,7 +255,7 @@ fn gpu_array_write_local
   (#sz: erased nat)
   (#i: erased nat)
   (#j: erased nat)
-  (r:gpu_array a sz)
+  (r:gpu_array_core a sz)
   (idx : SZ.t)
   (v : a)
   (#s : erased (seq a))
@@ -277,7 +277,7 @@ fn gpu_array_read_loc
   (#sz : erased nat)
   (#i  : erased nat)
   (#j  : erased nat)
-  (r : gpu_array a sz)
+  (r : gpu_array_core a sz)
   (#f : perm)
   (idx : SZ.t)
   (#s : erased (seq a))
@@ -306,7 +306,7 @@ fn gpu_array_write_loc
   (#sz: erased nat)
   (#i: erased nat)
   (#j: erased nat)
-  (r:gpu_array a sz)
+  (r:gpu_array_core a sz)
   (idx : SZ.t)
   (v : a)
   (#s : erased (seq a))
@@ -330,13 +330,13 @@ fn gpu_array_write_loc
 
 
 [@@noextract_to "krml"]
-fn gpu_global_array_read
+fn gpu_array_read
   (#a : Type u#0)
   (#sz : erased nat)
   (#i  : erased nat)
   (#j  : erased nat)
   (#gpu_id : erased int)
-  (r : gpu_global_array #gpu_id a sz)
+  (r : gpu_array #gpu_id a sz)
   (#f : perm)
   (idx : SZ.t)
   (#s : erased (seq a))
@@ -355,13 +355,13 @@ fn gpu_global_array_read
 }
 
 [@@noextract_to "krml"]
-fn gpu_global_array_write
+fn gpu_array_write
   (#a:Type u#0)
   (#sz: erased nat)
   (#i: erased nat)
   (#j: erased nat)
   (#gpu_id : erased int)
-  (r:gpu_global_array #gpu_id a sz)
+  (r:gpu_array #gpu_id a sz)
   (idx : SZ.t)
   (v : a)
   (#s : erased (seq a))
@@ -385,14 +385,14 @@ fn gpu_shmem_array_read
   (#sz : erased nat)
   (#i  : erased nat)
   (#j  : erased nat)
-  (r : gpu_shmem_array a sz)
+  (#gpu_id #nblk #bid:erased int)
+  (r:gpu_shmem_array #gpu_id bid a sz)
   (#f : perm)
   (idx : SZ.t)
   (#s : erased (seq a))
-  (#gpu_id #nblk #bid:erased int)
   preserves block_id #gpu_id nblk bid
   preserves gpu_pts_to_slice #a #sz r #f i j s
-  requires pure (i <= SZ.v idx /\ SZ.v idx < j /\ visible_on_block r gpu_id bid)
+  requires pure (i <= SZ.v idx /\ SZ.v idx < j)
   returns  x:a
   ensures  pure (i <= j /\ j <= sz /\ Seq.length s == (j-i) /\
                  i <= SZ.v idx /\ SZ.v idx < j /\
@@ -411,13 +411,13 @@ fn gpu_shmem_array_write
   (#sz: erased nat)
   (#i: erased nat)
   (#j: erased nat)
-  (r:gpu_shmem_array a sz)
+  (#gpu_id #nblk #bid:erased int)
+  (r:gpu_shmem_array #gpu_id bid a sz)
   (idx : SZ.t)
   (v : a)
   (#s : erased (seq a))
-  (#gpu_id #nblk #bid:erased int)
   preserves block_id #gpu_id nblk bid
-  requires pure (i <= SZ.v idx /\ SZ.v idx < j /\ visible_on_block r gpu_id bid)
+  requires pure (i <= SZ.v idx /\ SZ.v idx < j)
   requires gpu_pts_to_slice #a #sz r #1.0R i j s
   ensures
     with_pure
@@ -434,7 +434,7 @@ fn gpu_memcpy_host_to_device'
   {| sized a |}
   (#dst_sz : erased nat)
   (#gpu_id: erased int)
-  (dst_garr : gpu_global_array #gpu_id a dst_sz)
+  (dst_garr : gpu_array #gpu_id a dst_sz)
   (dst_off : SZ.t)
   (#src_sz : erased nat)
   (src_arr : vec a)
@@ -462,7 +462,7 @@ fn gpu_memcpy_host_to_device
   {| sized a |}
   (#sz : erased nat)
   (#gpu_id: erased int)
-  (dst_garr : gpu_global_array #gpu_id a sz)
+  (dst_garr : gpu_array #gpu_id a sz)
   (src_arr : vec a)
   (cnt : SZ.t)
   (#f : perm)
@@ -493,7 +493,7 @@ fn gpu_memcpy_device_to_host'
   (dst_off : SZ.t)
   (#src_sz : erased nat)
   (#gpu_id : erased int)
-  (src_garr : gpu_global_array #gpu_id a src_sz)
+  (src_garr : gpu_array #gpu_id a src_sz)
   (src_off : SZ.t)
   (cnt : SZ.t {
     dst_off + cnt <= dst_sz /\
@@ -520,7 +520,7 @@ fn gpu_memcpy_device_to_host
   (#sz : erased nat)
   (#gpu_id : erased int)
   (dst_arr : vec a)
-  (src_garr : gpu_global_array #gpu_id a sz)
+  (src_garr : gpu_array #gpu_id a sz)
   (cnt : SZ.t)
   (#f : perm)
   (#v : erased (seq a))
@@ -546,8 +546,8 @@ fn gpu_memcpy_device_to_device
   {| sized a |}
   (#sz : erased nat)
   (#gpu1 #gpu2:erased int)
-  (dst_arr : gpu_global_array #gpu1 a sz)
-  (src_garr : gpu_global_array #gpu2 a sz)
+  (dst_arr : gpu_array #gpu1 a sz)
+  (src_garr : gpu_array #gpu2 a sz)
   (cnt : SZ.t)
   (#f : perm)
   (#v : erased (seq a))
@@ -570,7 +570,7 @@ ghost
 fn gpu_array_slice_1
   (#a:Type u#0)
   (#sz:nat)
-  (arr : gpu_array a sz)
+  (arr : gpu_array_core a sz)
   (#f : perm)
   (#v : erased (seq a) { Seq.length v == sz })
   requires pts_to arr #f v
@@ -583,7 +583,7 @@ ghost
 fn gpu_array_unslice_1
   (#a:Type u#0)
   (#sz:nat)
-  (arr : gpu_array a sz)
+  (arr : gpu_array_core a sz)
   (#f : perm)
   (#v : erased (seq a) { Seq.length v == sz })
   requires forall+ (i: natlt sz). gpu_pts_to_cell arr #f i (v @! i)
@@ -597,7 +597,7 @@ ghost
 fn gpu_slice_concat
   (#a:Type u#0)
   (#sz:nat)
-  (arr : gpu_array a sz)
+  (arr : gpu_array_core a sz)
   (#[exact (`1.0R)] f : perm)
   (#s1 #s2: erased (seq a))
   (i n m:nat)
@@ -611,7 +611,7 @@ ghost
 fn gpu_slice_split
   (#a:Type u#0)
   (#sz:nat)
-  (arr : gpu_array a sz)
+  (arr : gpu_array_core a sz)
   (#[exact (`1.0R)] f : perm)
   (#s1 #s2: erased (seq a))
   (i n m:nat)
@@ -624,7 +624,7 @@ fn gpu_slice_split
 ghost
 fn gpu_slice_empty_elim
   (#a:Type u#0) (#sz:nat)
-  (arr : gpu_array a sz)
+  (arr : gpu_array_core a sz)
   (i : nat)
   requires gpu_pts_to_slice arr #'f i i 'v
   ensures  emp
@@ -635,7 +635,7 @@ fn gpu_slice_empty_elim
 ghost
 fn gpu_slice_empty_intro
   (#a:Type u#0) (#sz:nat)
-  (arr : gpu_array a sz)
+  (arr : gpu_array_core a sz)
   (i : nat)
   requires emp
   ensures  gpu_pts_to_slice arr #'f i i seq![]
@@ -647,7 +647,7 @@ ghost
 fn gpu_slice_share
   (#a:Type u#0)
   (#sz:nat)
-  (arr : gpu_array a sz)
+  (arr : gpu_array_core a sz)
   (m n:nat)
   (k: nat { k > 0 })
   (#f : perm)
@@ -662,7 +662,7 @@ ghost
 fn gpu_slice_gather
   (#a:Type u#0)
   (#sz:nat)
-  (arr : gpu_array a sz)
+  (arr : gpu_array_core a sz)
   (m n:nat)
   (k: nat { k > 0 })
   (#f : perm) // FIXME: if we use 'f, it gets type 'real' instead of 'perm'
@@ -677,7 +677,7 @@ ghost
 fn gpu_slice_pts_to_eq
   (#a:Type u#0)
   (#sz:nat)
-  (arr : gpu_array a sz)
+  (arr : gpu_array_core a sz)
   (m n:nat)
   (#f1 f2 : perm)
   (#v1 #v2 : seq a)
@@ -694,21 +694,21 @@ fn gpu_slice_pts_to_eq
 // val adjacent
 //   (#a : Type u#0)
 //   (#s1 #s2 : nat)
-//   (arr1 : gpu_array a s1)
-//   (arr2 : gpu_array a s2)
+//   (arr1 : gpu_array_core a s1)
+//   (arr2 : gpu_array_core a s2)
 //   : slprop
 
 // ghost
 // fn gpu_array_cut
 //   (#a : Type u#0) {| sized a |}
 //   (#sz : nat)
-//   (arr : gpu_array a sz)
+//   (arr : gpu_array_core a sz)
 //   (k : SZ.t{ k <= sz })
 //   (#s : lseq a sz)
 //   requires
 //     (arr |-> Frac 'f s)
 //   returns
-//     p : (gpu_array a k & gpu_array a (sz - k))
+//     p : (gpu_array_core a k & gpu_array_core a (sz - k))
 //   ensures
 //     (p._1 |-> Frac 'f (seq_take k s)) **
 //     (p._2 |-> Frac 'f (seq_drop k s)) **
@@ -722,13 +722,13 @@ fn gpu_slice_pts_to_eq
 // fn gpu_array_paste
 //   (#a : Type u#0)
 //   (#sz1 #sz2 : nat)
-//   (arr1 : gpu_array a sz1)
-//   (arr2 : gpu_array a sz2)
+//   (arr1 : gpu_array_core a sz1)
+//   (arr2 : gpu_array_core a sz2)
 //   requires
 //     (arr1 |-> Frac 'f 's1) **
 //     (arr2 |-> Frac 'f 's2) **
 //     adjacent arr1 arr2
 //   returns
-//     arr : gpu_array a (sz1 + sz2)
+//     arr : gpu_array_core a (sz1 + sz2)
 //   ensures
 //     arr |-> Frac 'f ('s1 @+ 's2)
