src/lib/kuiper/Kuiper.SHMem.fst
@@ -5,6 +5,7 @@ module Kuiper.SHMem
 open Pulse.Lib.Core
 open Kuiper.Array
 module SZ = Kuiper.SizeT
+module T = FStar.Tactics
 
 (* Description of one shared memory array "request" *)
 noeq
@@ -17,24 +18,24 @@ type shmem_desc =
     shmem_desc
 
 inline_for_extraction unfold
-let c_shmem (d : shmem_desc) : Type0 =
+let c_shmem (d : shmem_desc) (#[T.exact (`0)]gpu_id:int) (bid:int) : Type0 =
   match d with
-  | SHArray ty len -> gpu_array ty len
+  | SHArray ty len -> gpu_shmem_array #gpu_id bid ty len
 
 inline_for_extraction
-let rec c_shmems (d : list shmem_desc) : Type0 =
+let rec c_shmems (d : list shmem_desc) (#[T.exact (`0)]gpu_id:int) (bid:int) : Type0 =
   match d with
   | [] -> int // This could (and should) be unit, but karamel extraction gets confused with it
   | d :: ds ->
-    c_shmem d & c_shmems ds
+    c_shmem d #gpu_id bid & c_shmems ds #gpu_id bid
 
-let live_c_shmem #d (c : c_shmem d) : slprop =
+let live_c_shmem #d #gpu_id #bid (c : c_shmem d #gpu_id bid) : slprop =
   match d with
   | SHArray ty len -> exists* v. gpu_pts_to_array #ty #len c #1.0R v
 
-let rec live_c_shmems #ds (c : c_shmems ds) : slprop =
+let rec live_c_shmems #ds #gpu_id #bid (c : c_shmems ds #gpu_id bid) : slprop =
   match ds with
   | [] -> emp
   | d :: ds ->
-    let c : c_shmem d & c_shmems ds = c in (* coerce *)
-    live_c_shmem #d (fst c) ** live_c_shmems #ds (snd c)
+    let c : c_shmem d #gpu_id bid & c_shmems ds #gpu_id bid = c in (* coerce *)
+    live_c_shmem #d #gpu_id #bid (fst c) ** live_c_shmems #ds #gpu_id #bid (snd c)
