src/lib/poly/Kuiper.Poly.Softmax.fsti
@@ -27,7 +27,7 @@ let softmax_real (s:Seq.seq real { Seq.length s > 0 }) =
 unfold
 type softmax_gpu_ty (et : Type0) {| floating et, real_like et |} =
   (#lena : szp { lena < max_threads }) ->
-  (a : gpu_global_array et lena) ->
+  (a : gpu_array et lena) ->
   (#va : erased (seq et)) ->
   (#ra : erased (seq real) { Seq.length ra == SizeT.v lena /\ va %~ ra /\ lena > 0 }) ->
   stt unit
