src/lib/poly/gemm/Kuiper.Poly.GEMM.Tiled.Common.fsti
@@ -50,12 +50,13 @@ fn copy_tiles_out_of_matrices
   (nthr : sz)
   (#_ : squash (SZ.fits (bm*bk + nthr-1)))
   (#_ : squash (SZ.fits (bk*bn + nthr-1)))
+  (#bid : erased int)
   (tid : szlt nthr)
   preserves
     gpu **
     gA |-> Frac fA eA **
     gB |-> Frac fB eB **
-    thread_id nthr tid **
+    thread_id nthr bid tid **
     live_strided_chunks sA nthr tid **
     live_strided_chunks sB nthr tid
 
